\documentclass[a5paper]{article}
\input{./exercise-header.tex}
\begin{document}
\title{HoTT: Exercise 2.1.2}
\author{Langston Barrett}
\date{Fall 2017}

\begin{lemma*}[Lemma 2.1.2]
	For every type $A$ and every $x,y,z:A$ there is a function
  \begin{equation*}
    (x=y)\longrightarrow (y=z)\longrightarrow (x=z)
  \end{equation*}
  % Equivalently, the following type is inhabited:
  % \begin{equation*}
  %   \prod_{A:U}\prod_{x,y,z:A}(x=y)\to (y=z)\to (x=z)
  % \end{equation*}
\end{lemma*}
\begin{proof}[Proof 2: Induction on $p$]
	Define 
  \begin{gather*}
    D:\prod_{(x,y:A)}(x=y)\to U \\
    D(x,y,p):\equiv\prod_{(z:A)}\prod_{(q:y=z)} (x=z)
  \end{gather*}
  Then
  \begin{equation*}
    D(x,x,\refl_x)\equiv \prod_{(z:A)}\prod_{(q:x=z)}(x=z)
  \end{equation*}
  Thus, we have
  \begin{equation*}
    d:\equiv\lambda x.\lambda z.\lambda q.q : \prod_{(x:A)} D(x,x,\refl_x)
  \end{equation*}
  So by induction, we have a function
  \begin{equation*}
    f:\prod_{(x,y:A)}\prod_{(p:x=y)} D(x,y,p)\equiv\prod_{(x,y:A)}\prod_{(p:x=y)}\prod_{(z:A)}\prod_{(q:y=z)}(x=z)
  \end{equation*}
  such that 
  \begin{equation*}
    f(x,x,\refl_x)\equiv \lambda z.\lambda q.q
  \end{equation*}
  In summary, we make the following judgement:
  \begin{multline*}
    \ind_{=_A}\Big({\prod_{(z:A)}\prod_{(q:y=z)} (x=z)},
    {\lambda x.\lambda z.\lambda q.q}\Big) \\
    :\prod_{(x,y:A)}\prod_{(p:x=y)}\prod_{(z:A)}\prod_{(q:y=z)}(x=z)
  \end{multline*}
\end{proof}

\begin{proof}[Proof 3: Induction on $q$]
	Define 
  \begin{gather*}
    D:\prod_{(y,z:A)}(y=z)\to U \\
    D(y,z,p):\equiv\prod_{(x:A)}\prod_{(q:x=y)} (x=z)
  \end{gather*}
  Then
  \begin{equation*}
    D(y,y,\refl_y)\equiv \prod_{(x:A)}\prod_{(q:x=y)}(x=y)
  \end{equation*}
  Thus, we have
  \begin{equation*}
    d:\equiv\lambda y.\lambda x.\lambda q.q : \prod_{(y:A)} D(y,y,\refl_y)
  \end{equation*}
  So by induction, we have a function
  \begin{equation*}
    f:\prod_{(y,z:A)}\prod_{(p:y=z)} D(y,z,p)
    \equiv\prod_{(y,z:A)}\prod_{(p:y=z)}\prod_{(x:A)}\prod_{(q:x=y)} (x=z)
  \end{equation*}
  such that 
  \begin{equation*}
    f(y,y,\refl_y)\equiv \lambda x.\lambda q.q
  \end{equation*}
  In summary, we make the following judgement:
  \begin{multline*}
    \ind_{=_A}\Big(\prod_{(x:A)}\prod_{(q:x=y)}(x=y),
    y.\lambda x.\lambda q.q\Big) \\
    :\prod_{(y,z:A)}\prod_{(p:y=z)}\prod_{(x:A)}\prod_{(q:x=y)} (x=z)
  \end{multline*}
\end{proof}

The first proof, namely the one involving induction on both $p$ and $q$ appears
in the text.

\end{document}